theories/compiler/monads.v
@@ -1,0 +1,163 @@
+From stdpp Require Import base strings gmap gmultiset fin_sets decidable.
+From Wasm Require datatypes.
+From RWasm Require Import exn state.
+From RWasm Require Export exn state.
+(* ExtLib has its own state monad but it doens't play nicely with stdpp *)
+Definition state (S A : Type) : Type := S -> (S * A).
+
+(* Not great but ok for now *)
+Inductive Err :=
+| err (msg: string).
+
+(* The compiler monad. *)
+#[global]
+Definition M := exn Err.
+
+Definition mlookup_with_msg {A} (idx: nat) (lst: list A) (msg: string) : M A :=
+  match list_lookup idx lst with
+  | Some x => mret x
+  | None => mthrow (err msg)
+  end.
+
+Module wasm := datatypes.
+Section TempLocals.
+
+  Context `{!EqDecision wasm.value_type}.
+
+  #[global]
+  Instance wasm_value_type_eq_dec : EqDecision wasm.value_type.
+  Proof.
+    unfold EqDecision.
+    intros x y.
+    destruct x; destruct y;
+      (left; reflexivity) || (right; discriminate).
+  Defined.
+
+  Record TempLocals := {
+    tl_start : nat;
+    tl_next  : nat;
+    tl_types : gmap nat datatypes.value_type;
+    tl_free  : gset nat
+  }.
+
+  Definition new_tl (start : nat) : TempLocals :=
+    {| tl_start := start; tl_next := start; tl_types := ∅; tl_free := ∅ |}.
+  Definition InstM := stateT TempLocals M.
+  Definition get_st  : InstM TempLocals               := mget.
+  Definition put_st  : TempLocals → InstM unit        := mput.
+  Definition modify_st (f : TempLocals → TempLocals)  : InstM unit := mmodify f.
+  Definition lift_M {A} (m : M A) : InstM A :=
+    λ st,
+      x ← m;
+      mret (st, x).
+  Definition fresh_local (ty : wasm.value_type) : InstM wasm.immediate :=
+    st ← get_st;
+    let reusable := filter (λ i, tl_types st !! i = Some ty) (elements (tl_free st)) in
+    match reusable with
+    | i :: _ =>
+      let st' :=
+        {| tl_start := tl_start st;
+           tl_next  := tl_next st;
+           tl_types := tl_types st;
+           tl_free  := tl_free st ∖ {[ i ]} |} in
+      put_st st';;
+      mret i
+    | [] =>
+      let i := tl_next st in
+      let st' :=
+        {| tl_start := tl_start st;
+           tl_next  := S i;
+           tl_types := <[ i := ty ]> (tl_types st);
+           tl_free  := tl_free st |} in
+      put_st st';;
+      mret i
+    end.
+  Definition free_local (i : wasm.immediate) : InstM unit :=
+    modify_st (λ st, {| tl_start := tl_start st;
+                        tl_next  := tl_next  st;
+                        tl_types := tl_types st;
+                        tl_free  := tl_free  st ∪ {[ i ]} |}).
+End TempLocals.
+
+Section Example.
+  Context `{!EqDecision wasm.value_type}.
+
+  Let st0 : TempLocals :=
+    {| tl_start := 5;
+       tl_next := 5;
+       tl_types := ∅;
+       tl_free := ∅ |}.
+
+  Let tmp1 := match fresh_local wasm.T_i32 st0 with | OK (st1, i1) => (st1, i1) | _ => (st0, 0) end.
+  Let st1 := fst tmp1.
+  Let i1 := snd tmp1.
+
+  Let tmp2 := match fresh_local wasm.T_f64 st1 with | OK (st2, i2) => (st2, i2) | _ => (st1, 0) end.
+  Let st2 := fst tmp2.
+  Let i2 := snd tmp2.
+
+  Let tmp3 := match free_local i1 st2 with | OK (s,_) => s | _ => st2 end.
+  Let st3 := tmp3.
+
+  Let tmp4 := match fresh_local wasm.T_i32 st3 with | OK (st4, i3) => (st4, i3) | _ => (st3, 0) end.
+  Let st4 := fst tmp4.
+  Let i3 := snd tmp4.
+
+  Goal True.
+    assert (tl_types st4 !! i1 = Some wasm.T_i32) by (cbn; reflexivity).
+    assert (tl_types st4 !! i2 = Some wasm.T_f64) by (cbn; reflexivity).
+    assert (tl_types st4 !! i3 = Some wasm.T_i32)by (cbn; reflexivity).
+    assert (i3 = i1) by reflexivity.
+
+    exact I.
+  Qed.
+
+End Example.
+
+Lemma stateT_bind_OK_inv
+      {S A B}
+      (m : stateT S (exn Err) A)
+      (f : A → stateT S (exn Err) B)
+      (s : S) (st' : S) (b : B) :
+  (m ≫= f) s = @OK Err (S * B) (st', b) →
+  ∃ st1 a, m s = OK Err (S * A) (st1, a) ∧ f a st1 = OK Err (S * B) (st', b).
+Proof.
+  unfold mbind, stateT_MBind; simpl.
+  destruct (m s) as [e | [st1 a]] eqn:Hm; simpl.
+  - intros H. discriminate H.
+  - intros H. exists st1, a. split; [rewrite <- Hm | exact H]. reflexivity.
+Qed.
+
+Lemma fresh_local_preserves_tl_types ty st st' i :
+  fresh_local ty st = mret (st', i) →
+  tl_types st' !! i = Some ty
+  /\
+  (∀ j t, tl_types st !! j = Some t → tl_types st' !! j = Some t).
+Proof.
+  unfold fresh_local, get_st; cbn.
+  intro Hrun.
+    remember (filter (λ j, tl_types st !! j = Some ty)
+                   (elements (tl_free st))) as reusable eqn:Heq.
+  destruct reusable as [k |] eqn:Hr; cbn in Hrun.
+    - admit.
+    - admit.
+Admitted.
+
+(* TODO: this feels like it should already exist in stdpp *)
+Section monadic_fold.
+  Context {M : Type → Type}.
+  Context `{!MBind M, !MRet M}.
+
+  Fixpoint foldrM {A B} (f : A → B → M B) (init : B) (l : list A) : M B :=
+    match l with
+    | [] => mret init
+    | x :: xs => foldrM f init xs ≫= fun acc => f x acc
+    end.
+
+  Fixpoint foldlM {A B} (f : A → B → M B) (init : B) (l : list A) : M B :=
+    match l with
+    | [] => mret init
+    | x :: xs => f x init ≫= fun acc => foldlM f acc xs
+    end.
+End monadic_fold.
+
